@prefix acqf-qcp-model: <https://data.acqf-acp.africa/model/> .
@prefix :               <https://data.acqf-acp.africa/model/acqf-levels/resource/> .
@prefix dct:            <http://purl.org/dc/terms/> .
@prefix rdf:            <http://www.w3.org/1999/02/22-rdf-syntax-ns#> .
@prefix skos:           <http://www.w3.org/2004/02/skos/core#> .
@prefix xsd:            <http://www.w3.org/2001/XMLSchema#> .

acqf-qcp-model:acqf-levels
    a                  skos:ConceptScheme ;
    dct:title          "ACQF levels and level descriptors"@en ;
    dct:description    "This is a SKOS representation of the ACQF levels and level descriptors."@en ;
    dct:created        "2024-06-25"^^xsd:date ;
    dct:created        "2024-06-25"^^xsd:date ;
    dct:created        "2024-06-25"^^xsd:date ;
    dct:publisher      "cognizone bv" ;
    dct:creator        "Petr KÅ™emen" ;
    dct:license        <http://creativecommons.org/publicdomain/zero/1.0/> ;
    dct:source         <https://acqf.africa/resources/policy-guidelines/acqf-level-descriptors/acqf-level-descriptors-article-newsletter-1-march-2022/@@display-file/file/ACQF_CDP%2010_Level%20descriptors_Article%20Newsletter%201.pdf> ;
    skos:hasTopConcept :level-0, :level-1, :level-2, :level-3, :level-4, :level-5, :level-6, :level-7, :level-8,
                       :level-9 .

:level-1
    a               skos:Concept ;
    skos:inScheme   acqf-qcp-model:acqf-levels ;
    skos:prefLabel  "Level 1"@en ;
    skos:notation   "ACQF-1" ;
    skos:definition """The learning outcomes related to formal, non-formal and informal learning at this level include:

Knowledge (facts, principles and theories in various areas):
- simple knowledge, literacy and numeracy.

Skills (ability to use knowledge to respond to information and address problems. Skills include cognitive, communication, digital, green, innovation, practical and social skills):
- simple communication, cognitive and practical skills required to follow simple instructions, and use simple, repetitive solutions to address simple problems.

Autonomy and responsibility (context and extent of the application of autonomy and responsibility):
- highly structured, repetitive contexts under close supervision and guidance taking minimal responsibility for self."""
.

:level-2
    a               skos:Concept ;
    skos:inScheme   acqf-qcp-model:acqf-levels ;
    skos:prefLabel  "Level 2"@en ;
    skos:notation   "ACQF-2" ;
    skos:definition """The learning outcomes related to formal, non-formal and informal learning at this level include:

Knowledge (facts, principles and theories in various areas):
- basic knowledge incorporating comprehension and recall of factual and operational knowledge in some areas.

Skills (ability to use knowledge to respond to information and address problems. Skills include cognitive, communication, digital, green, innovation, practical and social skills):
- basic communication, cognitive and practical skills required to use concrete information, ideas and known solutions to address straightforward problems.

Autonomy and responsibility (context and extent of the application of autonomy and responsibility):
- structured contexts under limited supervision and guidance taking limited responsibility for self and group outcomes"""
.

:level-3
    a               skos:Concept ;
    skos:inScheme   acqf-qcp-model:acqf-levels ;
    skos:prefLabel  "Level 3"@en ;
    skos:notation   "ACQF-3" ;
    skos:definition """The learning outcomes related to formal, non-formal and informal learning at this level include:

Knowledge (facts, principles and theories in various areas):
- factual and operational knowledge incorporating some theoretical aspects in some areas.

Skills (ability to use knowledge to respond to information and address problems. Skills include cognitive, communication, digital, green, innovation, practical and social skills):
- a range of communication, cognitive, practical and technical skills required to interpret and communicate ideas and detailed information and select and use known solutions to address familiar problems.

Autonomy and responsibility (context and extent of the application of autonomy and responsibility):
- predictable contexts under routine supervision and guidance, with initiative for self-responsibility and some responsibility for group outcomes."""
.

:level-4
    a               skos:Concept ;
    skos:inScheme   acqf-qcp-model:acqf-levels ;
    skos:prefLabel  "Level 4"@en ;
    skos:notation   "ACQF-4" ;
    skos:definition """The learning outcomes related to formal, non-formal and informal learning at this level include:

Knowledge (facts, principles and theories in various areas):
- mainly factual, operational or technical knowledge incorporating theoretical aspects in one or more areas.

Skills (ability to use knowledge to respond to information and address problems. Skills include cognitive, communication, digital, green, innovation, practical and social skills):
- well-developed technical skills required to analyse information and new ideas, make informed judgements, communicate outcomes and apply varied solutions to varied (familiar and unfamiliar) problems.

Autonomy and responsibility (context and extent of the application of autonomy and responsibility):
- varied (predictable and unpredictable) contexts with adaptability and initiative for self-direction under general guidance, taking full responsibility for self, some planning and responsibility for group outcomes and initiative for responsibility for others."""
.

:level-5
    a               skos:Concept ;
    skos:inScheme   acqf-qcp-model:acqf-levels ;
    skos:prefLabel  "Level 5"@en ;
    skos:notation   "ACQF-5" ;
    skos:definition """The learning outcomes related to formal, non-formal and informal learning at this level include:

Knowledge (facts, principles and theories in various areas):
- mainly technical or theoretical knowledge with substantial depth in a discipline/ area.

Skills (ability to use knowledge to respond to information and address problems. Skills include cognitive, communication, digital, green, innovation, practical and social skills):
- a range of well-developed technical skills, with some specialisation, required to analyse information and new ideas, construct and communicate a coherent argument, and apply a range of solutions, often in combination, to address unfamiliar problems.

Autonomy and responsibility (context and extent of the application of autonomy and responsibility):
- unpredictable contexts with full autonomy and full responsibility for self and group outcomes, and some responsibility for others."""
.

:level-6
    a               skos:Concept ;
    skos:inScheme   acqf-qcp-model:acqf-levels ;
    skos:prefLabel  "Level 6"@en ;
    skos:notation   "ACQF-6" ;
    skos:definition """The learning outcomes related to formal, non-formal and informal learning at this level include:

Knowledge (facts, principles and theories in various areas):
- highly technical or theoretical knowledge, with specialisation in a discipline/ area.

Skills (ability to use knowledge to respond to information and address problems. Skills include cognitive, communication, digital, green, innovation, practical and social skills):
- highly technical and specialised skills required to collate, analyse, synthesise and communicate a range of information and new ideas, and formulate or adapt different solutions to address complex and sometimes abstract problems .

Autonomy and responsibility (context and extent of the application of autonomy and responsibility):
- highly variable contexts with well-developed autonomy and responsibility for self and group outcomes and responsibility for resources and processes."""
.


:level-7
    a               skos:Concept ;
    skos:inScheme   acqf-qcp-model:acqf-levels ;
    skos:prefLabel  "Level 7"@en ;
    skos:notation   "ACQF-7" ;
    skos:definition """The learning outcomes related to formal, non-formal and informal learning at this level include:

Knowledge (facts, principles and theories in various areas):
- advanced analytical and/ or specialised knowledge of a discipline/ area.

Skills (ability to use knowledge to respond to information and address problems. Skills include cognitive, communication, digital, green, innovation, practical and social skills):
- advanced, specialised skills required to demonstrate advanced analysis and initiative for new insights and ideas in research and/ or innovation, and formulate advanced solutions to address complex and abstract problems.

Autonomy and responsibility (context and extent of the application of autonomy and responsibility):
- complex and variable contexts with advanced autonomy and responsibility."""
.

:level-8
    a               skos:Concept ;
    skos:inScheme   acqf-qcp-model:acqf-levels ;
    skos:prefLabel  "Level 8"@en ;
    skos:notation   "ACQF-8" ;
    skos:definition """The learning outcomes related to formal, non-formal and informal learning at this level include:

Knowledge (facts, principles and theories in various areas):
- highly advanced, complex knowledge of a discipline/ area.

Skills (ability to use knowledge to respond to information and address problems. Skills include cognitive, communication, digital, green, innovation, practical and social skills):
- highly advanced, complex skills required to demonstrate highly advanced analysis, communicate new insights and ideas in research and/ or innovation, and formulate highly advanced solutions to address highly complex and abstract problems .

Autonomy and responsibility (context and extent of the application of autonomy and responsibility):
- highly complex contexts with some specialisation demonstrating highly advanced autonomy and responsibility."""
.

:level-9
    a               skos:Concept ;
    skos:inScheme   acqf-qcp-model:acqf-levels ;
    skos:prefLabel  "Level 9"@en ;
    skos:notation   "ACQF-9" ;
    skos:definition """The learning outcomes related to formal, non-formal and informal learning at this level include:

Knowledge (facts, principles and theories in various areas):
- mastery of a complex body of knowledge at the forefront of a discipline/ area.

Skills (ability to use knowledge to respond to information and address problems. Skills include cognitive, communication, digital, green, innovation, practical and social skills):
- skills mastery required to demonstrate originality and new insights in research and/ or innovation and formulate and test theories to show mastery of highly complex, abstract problems.

Autonomy and responsibility (context and extent of the application of autonomy and responsibility):
- highly specialised contexts demonstrating mastery in autonomy and responsibility."""
.

:level-10
    a               skos:Concept ;
    skos:inScheme   acqf-qcp-model:acqf-levels ;
    skos:prefLabel  "Level 10"@en ;
    skos:notation   "ACQF-10" ;
    skos:definition """The learning outcomes related to formal, non-formal and informal learning at this level include:

Knowledge (facts, principles and theories in various areas):
- substantial and original knowledge contribution that extends the forefront of a discipline/ area and/ or at the interface between disciplines/ areas.

Skills (ability to use knowledge to respond to information and address problems. Skills include cognitive, communication, digital, green, innovation, practical and social skills):
- expert skills and techniques that demonstrate innovation, interpretation and creation of new ideas required to critically evaluate, formulate and test theories to address emergent, new and critical problems.

Autonomy and responsibility (context and extent of the application of autonomy and responsibility):
- emergent new contexts demonstrating expertise in management of new ideas."""
.
