@prefix acqf-qcp-model: <https://data.acqf-qcp.africa/model/> .
@prefix :               <https://data.acqf-qcp.africa/model/isced-2011/resource/> .
@prefix dct:            <http://purl.org/dc/terms/> .
@prefix rdf:            <http://www.w3.org/1999/02/22-rdf-syntax-ns#> .
@prefix skos:           <http://www.w3.org/2004/02/skos/core#> .
@prefix xsd:            <http://www.w3.org/2001/XMLSchema#> .

acqf-qcp-model:isced-2011
    a                  skos:ConceptScheme ;
    dct:title          "ISCED 2011 levels of education"@en ;
    dct:description    "This is a SKOS representation of the ISCED 2011 levels of education."@en ;
    dct:created        "2024-06-25"^^xsd:date ;
    dct:publisher      "cognizone bv" ;
    dct:creator        "Petr Křemen" ;
    dct:license        <http://creativecommons.org/publicdomain/zero/1.0/> ;
    dct:source         <https://uis.unesco.org/sites/default/files/documents/international-standard-classification-of-education-isced-2011-en.pdf> ;
    skos:hasTopConcept :level-0, :level-1, :level-2, :level-3, :level-4, :level-5, :level-6, :level-7, :level-8,
                       :level-9 .

:level-0
    a               skos:Concept ;
    skos:inScheme   acqf-qcp-model:isced-2011 ;
    skos:prefLabel  "Early childhood education"@en ;
    skos:altLabel   "ISCED 2011 - Level 0"@en ;
    skos:notation   "ISCED2011-0" ;
    skos:definition """Programmes at ISCED level 0, or early childhood education, are typically designed with a holistic
        approach to support children’s early cognitive, physical, social and emotional development
and introduce young children to organized instruction outside of the family context. ISCED
level 0 refers to early childhood programmes that have an intentional education component.
These programmes aim to develop socio-emotional skills necessary for participation in school
and society. They also develop some of the skills needed for academic readiness and prepare
children for entry into primary education.

At this level, programmes are not necessarily highly structured but are designed to provide an
organized and purposeful set of learning activities in a safe physical environment. They allow
children to learn through interaction with other children under the guidance of staff/educators,
typically through creative and play-based activities.

ISCED level 0 programmes target children below the age of entry into ISCED level 1. There are
two categories of ISCED level 0 programmes: early childhood educational development and preprimary education. The former has educational content designed for younger children (in the age
range of 0 to 2 years), whilst the latter is designed for children from age 3 years to the start of
primary education.

Programmes classified at ISCED level 0 may be referred to in many ways, for example: early
childhood education and development, play school, reception, pre-primary, pre-school, or
educación inicial. For programmes provided in crèches, daycare centres, nurseries or guarderías,
it is important to ensure that they meet the ISCED level 0 classification criteria specified below.
For international comparability purposes, the term ‘early childhood education’ is used to label
ISCED level 0
"""@en .

:level-1
    a               skos:Concept ;
    skos:inScheme   acqf-qcp-model:isced-2011 ;
    skos:prefLabel  "Primary education"@en ;
    skos:altLabel   "ISCED 2011 - Level 1"@en ;
    skos:notation   "ISCED2011-1" ;
    skos:definition """Programmes at ISCED level 1, or primary education, are typically designed to provide students
with fundamental skills in reading, writing and mathematics (i.e. literacy and numeracy) and
establish a solid foundation for learning and understanding core areas of knowledge, personal
and social development, in preparation for lower secondary education. It focuses on learning at a
basic level of complexity with little, if any, specialisation.

Educational activities at ISCED level 1 (particularly in the early grades) are often organized around
units, projects or broad learning areas, often with an integrated approach rather than providing
instruction in specific subjects. Typically, there is one main teacher responsible for a group of
pupils who organizes the learning process, although a class may have more than one teacher,
especially for certain subjects or units.

Age is typically the only entry requirement at this level. The customary or legal age of entry is
usually not below 5 years old nor above 7 years old. This level typically lasts six years, although
its duration can range between four and seven years. Primary education typically lasts until
age 10 to 12 (see Paragraphs 132 to 134). Upon completion of primary education programmes,
children may continue their education at ISCED level 2 (lower secondary education).

Programmes classified at ISCED level 1 may be referred to in many ways, for example: primary
education, elementary education or basic education (stage 1 or lower grades if an education
system has one programme that spans ISCED levels 1 and 2). For international comparability
purposes the term ‘primary education’ is used to label ISCED level 1.
"""@en .

:level-2
    a               skos:Concept ;
    skos:inScheme   acqf-qcp-model:isced-2011 ;
    skos:prefLabel  "Lower secondary education"@en ;
    skos:altLabel   "ISCED 2011 - Level 2"@en ;
    skos:notation   "ISCED2011-2" ;
    skos:definition """Programmes at ISCED level 2, or lower secondary education, are typically designed to build on
the learning outcomes from ISCED level 1. Usually, the aim is to lay the foundation for lifelong
learning and human development upon which education systems may then expand further
educational opportunities. Some education systems may already offer vocational education
programmes at ISCED level 2 to provide individuals with skills relevant to employment.

Programmes at this level are usually organized around a more subject-oriented curriculum,
introducing theoretical concepts across a broad range of subjects. Teachers typically have
pedagogical training in specific subjects and, more often than at ISCED level 1, a class of
students may have several teachers with specialised knowledge of the subjects they teach.

ISCED level 2 begins after four to seven years of ISCED level 1 education, with six years of
ISCED level 1 being the most common duration. Students enter ISCED level 2 typically between
ages 10 and 13 (age 12 being the most common).

Programmes classified at ISCED level 2 may be referred to in many ways, for example:
secondary school (stage one/lower grades if there is one programme that spans ISCED levels 2
and 3), junior secondary school, middle school, or junior high school. If a programme spans
ISCED levels 1 and 2, the terms elementary education or basic school (stage two/upper grades)
are often used. For international comparability purposes, the term ‘lower secondary education’ is
used to label ISCED level 2."""@en .

:level-3
    a               skos:Concept ;
    skos:inScheme   acqf-qcp-model:isced-2011 ;
    skos:prefLabel  "Upper secondary education"@en ;
    skos:altLabel   "ISCED 2011 - Level 3"@en ;
    skos:notation   "ISCED2011-3" ;
    skos:definition """Programmes at ISCED level 3, or upper secondary education, are typically designed to
complete secondary education in preparation for tertiary education or provide skills relevant to
employment, or both.

Programmes at this level offer students more varied, specialised and in-depth instruction
than programmes at ISCED level 2. They are more differentiated, with an increased range of
options and streams available. Teachers are often highly qualified in the subjects or fields of
specialisation they teach, particularly in the higher grades.

ISCED level 3 begins after 8 to 11 years of education since the beginning of ISCED level 1. Pupils
enter this level typically between ages 14 and 16. ISCED level 3 programmes usually end 12 or
13 years after the beginning of ISCED level 1 (or around age 17 or 18), with 12 years being the
most widespread cumulative duration. However, exit from upper secondary education may range
across education systems from usually 11 to 13 years of education since the beginning of ISCED
level 1.

Programmes classified at ISCED level 3 may be referred to in many ways, for example:
secondary school (stage two/upper grades), senior secondary school, or (senior) high school.
For international comparability purposes the term ‘upper secondary education’ is used to label
ISCED level 3."""@en
.

:level-4
    a               skos:Concept ;
    skos:inScheme   acqf-qcp-model:isced-2011 ;
    skos:prefLabel  "Post-secondary non-tertiary education"@en ;
    skos:altLabel   "ISCED 2011 - Level 4"@en ;
    skos:notation   "ISCED2011-4" ;
    skos:definition """Post-secondary non-tertiary education provides learning experiences building on secondary
education, preparing for labour market entry as well as tertiary education. It aims at the
individual acquisition of knowledge, skills and competencies lower than the level of complexity
characteristic of tertiary education. Programmes at ISCED level 4, or post-secondary non-tertiary
education, are typically designed to provide individuals who completed ISCED level 3 with nontertiary qualifications required for progression to tertiary education or for employment when their
ISCED level 3 qualification does not grant such access. For example, graduates from general
ISCED level 3 programmes may choose to complete a non-tertiary vocational qualification; or
graduates from vocational ISCED level 3 programmes may choose to increase their level of
qualifications or specialise further. The content of ISCED level 4 programmes is not sufficiently
complex to be regarded as tertiary education, although it is clearly post-secondary.

The completion of an ISCED level 3 programme is required to enter ISCED level 4 programmes.
However, these entry requirements may be lower than for tertiary programmes at ISCED level 5,
6 or 7.

Usually, programmes at this level are designed for direct labour market entry. In some education
systems, there are general programmes at this level. Such programmes typically target students
who have completed ISCED level 3 but who want to increase their opportunities to enter tertiary
education.

Programmes classified at ISCED level 4 may be referred to in many ways, for example: technician
diploma, primary professional education, or préparation aux carrières administratives. For
international comparability purposes the term ‘post-secondary non-tertiary education’ is used to
label ISCED level 4.
"""@en .

:level-5
    a               skos:Concept ;
    skos:inScheme   acqf-qcp-model:isced-2011 ;
    skos:prefLabel  "Short-cycle tertiary education"@en ;
    skos:altLabel   "ISCED 2011 - Level 5"@en ;
    skos:notation   "ISCED2011-5" ;
    skos:definition """Programmes at ISCED level 5, or short-cycle tertiary education, are often designed to provide
participants with professional knowledge, skills and competencies. Typically, they are practicallybased, occupationally-specific and prepare students to enter the labour market. However, these
programmes may also provide a pathway to other tertiary education programmes. Academic
tertiary education programmes below the level of a Bachelor’s programme or equivalent are also
classified as ISCED level 5.

Entry into ISCED level 5 programmes requires the successful completion of ISCED level 3 or 4
with access to tertiary education. Programmes at ISCED level 5 have more complex content than
programmes at ISCED levels 3 and 4, but they are shorter and usually less theoretically-oriented
than ISCED level 6 programmes.

Although ISCED level 5 programmes are usually designed to prepare for employment, they may
give credit for transfer into ISCED level 6 or 7 programmes. Upon completion of these ISCED
level 5 programmes, individuals may in some education systems continue their education at
ISCED level 6 (Bachelor’s or equivalent level) or long first degree ISCED level 7 programmes
(Master’s or equivalent level).

Programmes classified at ISCED level 5 may be referred to in many ways, for example: (higher)
technical education, community college education, technician or advanced/higher vocational
training, associate degree, or bac+2. For international comparability purposes the term ‘shortcycle tertiary education’ is used to label ISCED level 5."""@en
.

:level-6
    a               skos:Concept ;
    skos:inScheme   acqf-qcp-model:isced-2011 ;
    skos:prefLabel  "Bachelor’s or equivalent level"@en ;
    skos:altLabel   "ISCED 2011 - Level 6"@en ;
    skos:notation   "ISCED2011-6" ;
    skos:definition """Programmes at ISCED level 6, or Bachelor’s or equivalent level, are often designed to provide
participants with intermediate academic and/or professional knowledge, skills and competencies,
leading to a first degree or equivalent qualification. Programmes at this level are typically
theoretically-based but may include practical components and are informed by state of the art
research and/or best professional practice. They are traditionally offered by universities and
equivalent tertiary educational institutions.

Instruction at this level often takes the form of lectures by staff who are typically required to have
attained ISCED levels 7 or 8 or have achieved experience as a senior professional in the field of
work. Programmes at this level do not necessarily involve the completion of a research project or
thesis, but if they do, it is less advanced, less independent or is undertaken with more guidance
than those at ISCED level 7 or 8.

Entry into these programmes normally requires the successful completion of an ISCED level 3
or 4 programme with access to tertiary education. Entry may depend on subject choice and/or
grades achieved at ISCED levels 3 and/or 4. Additionally, it may be required to take and succeed
in entry examinations. Entry or transfer into ISCED level 6 is also sometimes possible after
the successful completion of ISCED level 5. Upon completion of ISCED level 6 programmes,
individuals may continue their education at ISCED level 7 (Master’s or equivalent level), although
not all ISCED level 6 programmes provide access to ISCED level 7. ISCED level 6 programmes
do not usually give direct access to programmes at ISCED level 8 (doctoral or equivalent level).

Programmes classified at ISCED level 6 may be referred to in many ways, for example:
Bachelor’s programme, licence, or first university cycle. However, it is important to note that
programmes with a similar name to ‘bachelor’ should only be included in ISCED level 6 if they
satisfy the criteria described in Paragraph 228. For international comparability purposes the term
‘Bachelor’s or equivalent level’ is used to label ISCED level 6."""@en
.

:level-7
    a               skos:Concept ;
    skos:inScheme   acqf-qcp-model:isced-2011 ;
    skos:prefLabel  "Master’s or equivalent level"@en ;
    skos:altLabel   "ISCED 2011 - Level 7"@en ;
    skos:notation   "ISCED2011-7" ;
    skos:definition """ Programmes at ISCED level 7, or Master’s or equivalent level, are often designed to provide
participants with advanced academic and/or professional knowledge, skills and competencies,
leading to a second degree or equivalent qualification. Programmes at this level may have a
substantial research component but do not yet lead to the award of a doctoral qualification.
Typically, programmes at this level are theoretically-based but may include practical components
and are informed by state of the art research and/or best professional practice. They are
traditionally offered by universities and other tertiary educational institutions.

Instruction at this level often takes the form of lectures by staff who are typically required to have
attained ISCED levels 7 or 8. Programmes at this level may involve the completion of a research
project or thesis that is more advanced than those expected at ISCED level 6 and less advanced
than those expected at ISCED level 8.

Entry into ISCED level 7 programmes preparing for a second or further degree normally requires
the successful completion of an ISCED level 6 or 7 programme. In the case of long programmes
that prepare for a first degree equivalent to a Master’s degree, entry requires the successful
completion of an ISCED level 3 or 4 programme with access to tertiary education. Entry into such
programmes may depend on subject choice and/or grades achieved at ISCED levels 3
and/or 4. Additionally, it may be required to take and succeed in entry examinations. ISCED
level 7 programmes have a significantly more complex content than programmes at ISCED
level 6 and are usually more specialised. Upon completion, individuals may continue their
education at ISCED level 8 (doctoral-level education) although not all ISCED level 7 programmes
give direct access to ISCED level 8.

Programmes classified at ISCED level 7 may be referred to in many ways, for example: master
programmes or magister. However, it is important to note that programmes with a similar name
to ‘master’ should only be included in ISCED level 7 if they satisfy the criteria described in
Paragraph 245. For international comparability purposes the term ‘Master’s or equivalent level’ is
used to label ISCED level 7."""@en
.

:level-8
    a               skos:Concept ;
    skos:inScheme   acqf-qcp-model:isced-2011 ;
    skos:prefLabel  "Doctoral or equivalent level"@en ;
    skos:altLabel   "ISCED 2011 - Level 8"@en ;
    skos:notation   "ISCED2011-8" ;
    skos:definition """Programmes at ISCED level 8, or doctoral or equivalent level, are designed primarily to lead to an
advanced research qualification. Programmes at this ISCED level are devoted to advanced study
and original research and are typically offered only by research-oriented tertiary educational
institutions such as universities. Doctoral programmes exist in both academic and professional
fields.

ISCED level 8 usually concludes with the submission and defence of a thesis, dissertation
or equivalent written work of publishable quality, representing a significant contribution to
knowledge in the respective field of study. Therefore, these programmes are typically based on
research and not only on course work. In some education systems, ISCED level 8 programmes
contain very limited course work, or none at all, and individuals working towards a doctoral
degree engage in research mostly independently or in small groups with varying degrees
of supervision. In some education systems, doctoral research is undertaken by individuals
employed by the university as junior researchers or research assistants, in addition to their being
enrolled as doctoral students.

Entry into ISCED level 8 programmes or junior research positions normally requires the
successful completion of specific ISCED level 7 programmes. ISCED level 8 qualifications give
access to professions with high academic skill requirements and research posts in government
and industry, as well as research and teaching positions in educational institutions offering
education at ISCED levels 6, 7 and 8.

Programmes classified at ISCED level 8 may be referred to in many ways, for example: PhD,
DPhil, D.Lit, D.Sc, LL.D, Doctorate or similar terms. However, it is important to note that
programmes with a similar name to ‘doctor’ should only be included in ISCED level 8 if they
satisfy the criteria described in Paragraph 263. For international comparability purposes, the term
‘doctoral or equivalent level’ is used to label ISCED level 8.
"""@en
.

:level-9
    a              skos:Concept ;
    skos:inScheme  acqf-qcp-model:isced-2011 ;
    skos:prefLabel "Not elsewhere classified"@en ;
    skos:altLabel  "ISCED 2011 - Level 9"@en ;
    skos:notation  "ISCED2011-9" .